theories/Operational/Common/Step.v
@@ -7,12 +7,18 @@ Inductive OpEvent : Type :=
 | EvWakeup (j : JobId)
 | EvBlock (j : JobId)
 | EvComplete (j : JobId)
-| EvResched (c : CPU)
+| EvRequestResched (c : CPU)
+| EvRecvIPI (c : CPU)
+| EvChoose (c : CPU) (j : JobId)
 | EvDispatch (c : CPU) (j : JobId)
 | EvTick.
 
 Definition add_runnable (j : JobId) (st : OpState) : OpState :=
-  mkOpState (op_current st) (j :: op_runnable st) (op_need_resched st).
+  mkOpState
+    (op_current st)
+    (j :: op_runnable st)
+    (op_need_resched st)
+    (op_dispatch_target st).
 
 Fixpoint remove_job (j : JobId) (xs : list JobId) : list JobId :=
   match xs with
@@ -21,7 +27,11 @@ Fixpoint remove_job (j : JobId) (xs : list JobId) : list JobId :=
   end.
 
 Definition remove_runnable (j : JobId) (st : OpState) : OpState :=
-  mkOpState (op_current st) (remove_job j (op_runnable st)) (op_need_resched st).
+  mkOpState
+    (op_current st)
+    (remove_job j (op_runnable st))
+    (op_need_resched st)
+    (op_dispatch_target st).
 
 Definition clear_current_job (j : JobId) (st : OpState) : OpState :=
   mkOpState
@@ -31,22 +41,35 @@ Definition clear_current_job (j : JobId) (st : OpState) : OpState :=
        | None => None
        end)
     (op_runnable st)
-    (op_need_resched st).
+    (op_need_resched st)
+    (op_dispatch_target st).
 
 Definition set_current (c : CPU) (oj : option JobId) (st : OpState) : OpState :=
   mkOpState
     (fun c' => if Nat.eqb c' c then oj else op_current st c')
     (op_runnable st)
-    (op_need_resched st).
+    (op_need_resched st)
+    (op_dispatch_target st).
 
 Definition set_need_resched (c : CPU) (b : bool) (st : OpState) : OpState :=
   mkOpState
     (op_current st)
     (op_runnable st)
-    (fun c' => if Nat.eqb c' c then b else op_need_resched st c').
+    (fun c' => if Nat.eqb c' c then b else op_need_resched st c')
+    (op_dispatch_target st).
 
 Definition clear_need_resched (c : CPU) (st : OpState) : OpState :=
   set_need_resched c false st.
+
+Definition set_dispatch_target (c : CPU) (oj : option JobId) (st : OpState) : OpState :=
+  mkOpState
+    (op_current st)
+    (op_runnable st)
+    (op_need_resched st)
+    (fun c' => if Nat.eqb c' c then oj else op_dispatch_target st c').
+
+Definition clear_dispatch_target (c : CPU) (st : OpState) : OpState :=
+  set_dispatch_target c None st.
 
 Definition clear_current_and_request (j : JobId) (st : OpState) : OpState :=
   mkOpState
@@ -60,7 +83,8 @@ Definition clear_current_and_request (j : JobId) (st : OpState) : OpState :=
        match op_current st c with
        | Some j' => if Nat.eqb j' j then true else op_need_resched st c
        | None => op_need_resched st c
-       end).
+       end)
+    (op_dispatch_target st).
 
 Inductive op_step : OpState -> OpEvent -> OpState -> Prop :=
 | step_wakeup :
@@ -68,23 +92,36 @@ Inductive op_step : OpState -> OpEvent -> OpState -> Prop :=
       op_step st (EvWakeup j) (add_runnable j st)
 | step_block :
     forall st j,
+      op_job_running st j ->
       op_step st (EvBlock j) (clear_current_and_request j st)
 | step_complete :
     forall st j,
+      op_job_running st j ->
       op_step st (EvComplete j) (clear_current_and_request j st)
-| step_resched :
+| step_request_resched :
     forall st c,
-      op_step st (EvResched c) (set_need_resched c true st)
-| step_dispatch :
+      op_step st (EvRequestResched c) (set_need_resched c true st)
+| step_recv_ipi :
+    forall st c,
+      op_step st (EvRecvIPI c) (set_need_resched c true st)
+| step_choose :
     forall st c j,
       In j (op_runnable st) ->
+      op_dispatch_target st c = None ->
+      ~ op_job_dispatch_pending st j ->
+      op_step st (EvChoose c j) (set_dispatch_target c (Some j) st)
+| step_dispatch :
+    forall st c j,
+      op_dispatch_target st c = Some j ->
       op_current st c = None ->
       op_step st (EvDispatch c j)
         (clear_need_resched c
-           (mkOpState
-              (fun c' => if Nat.eqb c' c then Some j else op_current st c')
-              (remove_job j (op_runnable st))
-              (op_need_resched st)))
+           (clear_dispatch_target c
+              (mkOpState
+                 (fun c' => if Nat.eqb c' c then Some j else op_current st c')
+                 (remove_job j (op_runnable st))
+                 (op_need_resched st)
+                 (op_dispatch_target st))))
 | step_tick :
     forall st,
       op_step st EvTick st.
