theories/Operational/Common/StepLemmas.v
@@ -53,6 +53,24 @@ Proof.
       * exact IH.
 Qed.
 
+Lemma remove_job_preserves_member :
+  forall j x xs,
+    In x xs ->
+    x <> j ->
+    In x (remove_job j xs).
+Proof.
+  intros j x xs Hin Hneq.
+  induction xs as [|y ys IH]; simpl in *.
+  - contradiction.
+  - destruct Hin as [<-|Hin].
+    + destruct (Nat.eqb y j) eqn:Hxj.
+      * apply Nat.eqb_eq in Hxj. contradiction.
+      * left. reflexivity.
+    + destruct (Nat.eqb y j) eqn:Hy.
+      * apply IH; assumption.
+      * right. apply IH; assumption.
+Qed.
+
 Lemma op_job_running_current :
   forall st j,
     op_job_running st j ->
@@ -64,160 +82,19 @@ Qed.
 
 Definition op_step_sound_pre (st : OpState) (ev : OpEvent) : Prop :=
   match ev with
-  | EvWakeup j => ~ In j (op_runnable st) /\ ~ op_job_running st j
+  | EvWakeup j =>
+      ~ In j (op_runnable st) /\
+      ~ op_job_running st j /\
+      ~ op_job_dispatch_pending st j
   | _ => True
   end.
 
-Lemma add_runnable_preserves_struct_inv :
-  forall m st j,
-    op_struct_inv m st ->
-    ~ In j (op_runnable st) ->
-    ~ op_job_running st j ->
-    op_struct_inv m (add_runnable j st).
-Proof.
-  intros m st j Hinv Hnotin Hnotrunning.
-  destruct Hinv as [Hdup Hnodup Hsep].
-  constructor.
-  - exact Hdup.
-  - simpl. constructor; assumption.
-  - intros c j' Hlt Hcur.
-    simpl.
-    intros [Heq|Hin].
-    + subst j'.
-      apply Hnotrunning.
-      exists c. exact Hcur.
-    + eapply Hsep; eauto.
-Qed.
-
-Lemma clear_current_and_request_preserves_struct_inv :
-  forall m st j,
-    op_struct_inv m st ->
-    op_struct_inv m (clear_current_and_request j st).
-Proof.
-  intros m st j Hinv.
-  destruct Hinv as [Hdup Hnodup Hsep].
-  constructor.
-  - intros j' c1 c2 Hlt1 Hlt2.
-    intros Hcur1 Hcur2.
-    simpl in Hcur1, Hcur2.
-    destruct (op_current st c1) as [k1|] eqn:Hc1; try discriminate.
-    destruct (Nat.eqb k1 j) eqn:Ek1; try discriminate.
-    destruct (op_current st c2) as [k2|] eqn:Hc2; try discriminate.
-    destruct (Nat.eqb k2 j) eqn:Ek2; try discriminate.
-    inversion Hcur1; inversion Hcur2; subst.
-    eapply Hdup; eauto.
-  - simpl. apply remove_job_preserves_NoDup. exact Hnodup.
-  - intros c j' Hlt.
-    intros Hcur Hin.
-    simpl in Hcur.
-    destruct (op_current st c) as [k|] eqn:Hc; try discriminate.
-    destruct (Nat.eqb k j) eqn:Ek; try discriminate.
-    inversion Hcur; subst.
-    apply remove_job_in in Hin as [Hin' _].
-    eapply Hsep; eauto.
-Qed.
-
-Lemma set_need_resched_preserves_struct_inv :
-  forall m st c b,
-    op_struct_inv m st ->
-    op_struct_inv m (set_need_resched c b st).
-Proof.
-  intros m st c b [Hdup Hnodup Hsep].
-  constructor; simpl; assumption.
-Qed.
-
-Lemma dispatch_target_not_in_remove_job :
-  forall j xs,
-    ~ In j (remove_job j xs).
-Proof.
-  apply remove_job_not_in.
-Qed.
-
-Lemma dispatch_other_not_in_remove_job :
-  forall j j' xs,
-    j' <> j ->
-    ~ In j' xs ->
-    ~ In j' (remove_job j xs).
-Proof.
-  intros j j' xs Hneq Hnotin Hin.
-  apply remove_job_in in Hin as [Hin _].
-  contradiction.
-Qed.
-
-Lemma dispatch_preserves_struct_inv :
-  forall m st c j,
-    op_struct_inv m st ->
-    In j (op_runnable st) ->
-    op_current st c = None ->
-    c < m ->
-    op_struct_inv
-      m
-      (clear_need_resched c
-         (mkOpState
-            (fun c' => if Nat.eqb c' c then Some j else op_current st c')
-            (remove_job j (op_runnable st))
-            (op_need_resched st))).
-Proof.
-  intros m st c j Hinv Hin Hjnone Hltc.
-  destruct Hinv as [Hdup Hnodup Hsep].
-  constructor.
-  - intros j' c1 c2 Hlt1 Hlt2.
-    simpl.
-    destruct (Nat.eqb c1 c) eqn:Ec1, (Nat.eqb c2 c) eqn:Ec2;
-      intros Hcur1 Hcur2.
-    + apply Nat.eqb_eq in Ec1.
-      apply Nat.eqb_eq in Ec2.
-      lia.
-    + apply Nat.eqb_eq in Ec1.
-      apply Nat.eqb_neq in Ec2.
-      subst c1.
-      inversion Hcur1; subst j'.
-      exfalso.
-      eapply (Hsep c2 j); eauto.
-    + apply Nat.eqb_neq in Ec1.
-      apply Nat.eqb_eq in Ec2.
-      subst c2.
-      inversion Hcur2; subst j'.
-      exfalso.
-      eapply (Hsep c1 j); eauto.
-    + eapply Hdup; eauto.
-  - simpl. apply remove_job_preserves_NoDup. exact Hnodup.
-  - intros c' j' Hlt'.
-    intros Hcur Hin'.
-    simpl in Hcur.
-    destruct (Nat.eqb c' c) eqn:Ecc.
-    + apply Nat.eqb_eq in Ecc. subst c'.
-      inversion Hcur; subst j'.
-      exact (dispatch_target_not_in_remove_job j (op_runnable st) Hin').
-    + apply Nat.eqb_neq in Ecc.
-      eapply Hsep; eauto.
-      eapply remove_job_in in Hin' as [Hin'' _].
-      exact Hin''.
-Qed.
-
-Lemma op_step_preserves_struct_inv :
-  forall m st ev st',
-    op_struct_inv m st ->
-    op_step_sound_pre st ev ->
-    op_step st ev st' ->
-    (forall c j, ev = EvDispatch c j -> c < m) ->
-    op_struct_inv m st'.
-Proof.
-  intros m st ev st' Hinv Hpre Hstep Hdispatch_lt.
-  inversion Hstep; subst; clear Hstep.
-  - destruct Hpre as [Hnotin Hnotrunning].
-    apply add_runnable_preserves_struct_inv; assumption.
-  - apply clear_current_and_request_preserves_struct_inv; assumption.
-  - apply clear_current_and_request_preserves_struct_inv; assumption.
-  - apply set_need_resched_preserves_struct_inv; assumption.
-  - eapply dispatch_preserves_struct_inv; eauto using Hdispatch_lt.
-  - exact Hinv.
-Qed.
-
 Definition op_step_range_pre (m : nat) (ev : OpEvent) : Prop :=
   match ev with
+  | EvRequestResched c => c < m
+  | EvRecvIPI c => c < m
+  | EvChoose c _ => c < m
   | EvDispatch c _ => c < m
-  | EvResched c => c < m
   | _ => True
   end.
 
@@ -227,6 +104,221 @@ Definition op_step_placement_pre
   | EvDispatch c j => c < m /\ adm j c
   | _ => True
   end.
+
+Lemma add_runnable_preserves_struct_inv :
+  forall m st j,
+    op_struct_inv m st ->
+    ~ In j (op_runnable st) ->
+    ~ op_job_running st j ->
+    ~ op_job_dispatch_pending st j ->
+    op_struct_inv m (add_runnable j st).
+Proof.
+  intros m st j Hinv Hnotin Hnotrunning Hnotpending.
+  destruct Hinv as [Hdup Hnodup Hsep Hdispatchdup Hdispatchrun].
+  constructor.
+  - exact Hdup.
+  - simpl. constructor; assumption.
+  - intros c j' Hcur.
+    simpl.
+    intros [Heq|Hin].
+    + subst j'.
+      apply Hnotrunning.
+      exists c. exact Hcur.
+    + eapply Hsep; eauto.
+  - intros j' c1 c2 Hlt1 Hlt2 Ht1 Ht2.
+    eapply Hdispatchdup; eauto.
+  - intros c j' Hlt Ht.
+    simpl in Ht.
+    right.
+    eapply Hdispatchrun; eauto.
+Qed.
+
+Lemma clear_current_and_request_preserves_struct_inv :
+  forall m st j,
+    op_struct_inv m st ->
+    op_job_running st j ->
+    op_struct_inv m (clear_current_and_request j st).
+Proof.
+  intros m st j Hinv Hrunning.
+  destruct Hinv as [Hdup Hnodup Hsep Hdispatchdup Hdispatchrun].
+  destruct Hrunning as [crun Hrun].
+  constructor.
+  - intros j' c1 c2 Hlt1 Hlt2 Hcur1 Hcur2.
+    simpl in Hcur1, Hcur2.
+    destruct (op_current st c1) as [k1|] eqn:Hc1; try discriminate.
+    destruct (Nat.eqb k1 j) eqn:Ek1; try discriminate.
+    destruct (op_current st c2) as [k2|] eqn:Hc2; try discriminate.
+    destruct (Nat.eqb k2 j) eqn:Ek2; try discriminate.
+    inversion Hcur1; inversion Hcur2; subst.
+    eapply Hdup; eauto.
+  - simpl. apply remove_job_preserves_NoDup. exact Hnodup.
+  - intros c j'.
+    intros Hcur Hin.
+    simpl in Hcur.
+    destruct (op_current st c) as [k|] eqn:Hc; try discriminate.
+    destruct (Nat.eqb k j) eqn:Ek; try discriminate.
+    inversion Hcur; subst.
+    apply remove_job_in in Hin as [Hin' _].
+    eapply Hsep; eauto.
+  - intros j' c1 c2 Hlt1 Hlt2 Ht1 Ht2.
+    simpl in Ht1, Ht2.
+    eapply Hdispatchdup; eauto.
+  - intros c j' Hlt Ht.
+    simpl in Ht.
+    specialize (Hdispatchrun c j' Hlt Ht) as Hin.
+    assert (j' <> j).
+    { intros ->.
+      eapply Hsep in Hin; eauto. }
+    apply remove_job_preserves_member; assumption.
+Qed.
+
+Lemma set_need_resched_preserves_struct_inv :
+  forall m st c b,
+    op_struct_inv m st ->
+    op_struct_inv m (set_need_resched c b st).
+Proof.
+  intros m st c b [Hdup Hnodup Hsep Hdispatchdup Hdispatchrun].
+  constructor; simpl; assumption.
+Qed.
+
+Lemma choose_preserves_struct_inv :
+  forall m st c j,
+    op_struct_inv m st ->
+    In j (op_runnable st) ->
+    op_dispatch_target st c = None ->
+    ~ op_job_dispatch_pending st j ->
+    c < m ->
+    op_struct_inv m (set_dispatch_target c (Some j) st).
+Proof.
+  intros m st c j Hinv Hinj Hslot Hnotpending Hltc.
+  destruct Hinv as [Hdup Hnodup Hsep Hdispatchdup Hdispatchrun].
+  constructor.
+  - exact Hdup.
+  - exact Hnodup.
+  - intros c' j' Hcur.
+    simpl.
+    exact (Hsep c' j' Hcur).
+  - intros j' c1 c2 Hlt1 Hlt2 Ht1 Ht2.
+    simpl in Ht1, Ht2.
+    destruct (Nat.eqb c1 c) eqn:Ec1, (Nat.eqb c2 c) eqn:Ec2.
+    + apply Nat.eqb_eq in Ec1.
+      apply Nat.eqb_eq in Ec2.
+      lia.
+    + apply Nat.eqb_eq in Ec1.
+      apply Nat.eqb_neq in Ec2.
+      subst c1.
+      inversion Ht1; subst j'.
+      exfalso.
+      apply Hnotpending.
+      exists c2. exact Ht2.
+    + apply Nat.eqb_neq in Ec1.
+      apply Nat.eqb_eq in Ec2.
+      subst c2.
+      inversion Ht2; subst j'.
+      exfalso.
+      apply Hnotpending.
+      exists c1. exact Ht1.
+    + eapply Hdispatchdup; eauto.
+  - intros c' j' Hlt Ht.
+    simpl in Ht.
+    destruct (Nat.eqb c' c) eqn:Ecc.
+    + apply Nat.eqb_eq in Ecc. subst c'.
+      inversion Ht; subst.
+      exact Hinj.
+    + eapply Hdispatchrun; eauto.
+Qed.
+
+Lemma dispatch_preserves_struct_inv :
+  forall m st c j,
+    op_struct_inv m st ->
+    op_dispatch_target st c = Some j ->
+    op_current st c = None ->
+    c < m ->
+    op_struct_inv
+      m
+      (clear_need_resched c
+         (clear_dispatch_target c
+            (mkOpState
+               (fun c' => if Nat.eqb c' c then Some j else op_current st c')
+               (remove_job j (op_runnable st))
+               (op_need_resched st)
+               (op_dispatch_target st)))).
+Proof.
+  intros m st c j Hinv Htarget Hnone Hltc.
+  destruct Hinv as [Hdup Hnodup Hsep Hdispatchdup Hdispatchrun].
+  constructor.
+  - intros j' c1 c2 Hlt1 Hlt2 Hcur1 Hcur2.
+    simpl in Hcur1, Hcur2.
+    destruct (Nat.eqb c1 c) eqn:Ec1, (Nat.eqb c2 c) eqn:Ec2.
+    + apply Nat.eqb_eq in Ec1.
+      apply Nat.eqb_eq in Ec2.
+      lia.
+    + apply Nat.eqb_eq in Ec1.
+      apply Nat.eqb_neq in Ec2.
+      subst c1.
+      inversion Hcur1; subst j'.
+      exfalso.
+      pose proof (Hdispatchrun c j Hltc Htarget) as Hinj.
+      eapply Hsep in Hinj; eauto.
+    + apply Nat.eqb_neq in Ec1.
+      apply Nat.eqb_eq in Ec2.
+      subst c2.
+      inversion Hcur2; subst j'.
+      exfalso.
+      pose proof (Hdispatchrun c j Hltc Htarget) as Hinj.
+      eapply Hsep in Hinj; eauto.
+    + eapply Hdup; eauto.
+  - simpl. apply remove_job_preserves_NoDup. exact Hnodup.
+  - intros c' j' Hcur Hin'.
+    simpl in Hcur.
+    destruct (Nat.eqb c' c) eqn:Ecc.
+    + apply Nat.eqb_eq in Ecc. subst c'.
+      inversion Hcur; subst j'.
+      exact (remove_job_not_in j (op_runnable st) Hin').
+    + apply Nat.eqb_neq in Ecc.
+      eapply Hsep; eauto.
+      apply remove_job_in in Hin' as [Hin'' _].
+      exact Hin''.
+  - intros j' c1 c2 Hlt1 Hlt2 Ht1 Ht2.
+    simpl in Ht1, Ht2.
+    destruct (Nat.eqb c1 c) eqn:Ec1, (Nat.eqb c2 c) eqn:Ec2; try discriminate.
+    eapply Hdispatchdup; eauto.
+  - intros c' j' Hlt' Ht.
+    simpl in Ht.
+    destruct (Nat.eqb c' c) eqn:Ecc.
+    + discriminate.
+    + assert (Hin_old : In j' (op_runnable st)).
+      { eapply Hdispatchrun; eauto. }
+      assert (j' <> j).
+      { intros Heq.
+        subst j'.
+        apply Nat.eqb_neq in Ecc.
+        pose proof (Hdispatchdup j c c' Hltc Hlt' Htarget Ht) as Heqcc.
+        lia.
+      }
+      apply remove_job_preserves_member; assumption.
+Qed.
+
+Lemma op_step_preserves_struct_inv :
+  forall m st ev st',
+    op_struct_inv m st ->
+    op_step_sound_pre st ev ->
+    op_step_range_pre m ev ->
+    op_step st ev st' ->
+    op_struct_inv m st'.
+Proof.
+  intros m st ev st' Hinv Hpre Hrange Hstep.
+  inversion Hstep; subst; clear Hstep.
+  - destruct Hpre as [Hnotin [Hnotrunning Hnotpending]].
+    apply add_runnable_preserves_struct_inv; assumption.
+  - eapply clear_current_and_request_preserves_struct_inv; eauto.
+  - eapply clear_current_and_request_preserves_struct_inv; eauto.
+  - apply set_need_resched_preserves_struct_inv; assumption.
+  - apply set_need_resched_preserves_struct_inv; assumption.
+  - eapply choose_preserves_struct_inv; eauto.
+  - eapply dispatch_preserves_struct_inv; eauto.
+  - exact Hinv.
+Qed.
 
 Lemma op_step_preserves_idle_outside_range :
   forall m st ev st',
@@ -239,20 +331,23 @@ Proof.
   inversion Hstep; subst; clear Hstep; simpl.
   - exact (Hid c Hge).
   - destruct (op_current st c) as [j'|] eqn:Hcur; simpl.
-    + pose proof (Hid c Hge) as Hnone.
-      rewrite Hcur in Hnone.
+    + pose proof (Hid c Hge) as Hnone0.
+      rewrite Hcur in Hnone0.
       discriminate.
     + reflexivity.
   - destruct (op_current st c) as [j'|] eqn:Hcur; simpl.
-    + pose proof (Hid c Hge) as Hnone.
-      rewrite Hcur in Hnone.
+    + pose proof (Hid c Hge) as Hnone0.
+      rewrite Hcur in Hnone0.
       discriminate.
     + reflexivity.
   - exact (Hid c Hge).
-  - simpl in Hpre.
-    destruct (Nat.eqb c c0) eqn:Ecc.
+  - exact (Hid c Hge).
+  - exact (Hid c Hge).
+  - destruct (Nat.eqb c c0) eqn:Ecc.
     + apply Nat.eqb_eq in Ecc. subst c.
-      exfalso. lia.
+      exfalso.
+      simpl in Hpre.
+      lia.
     + exact (Hid c Hge).
   - exact (Hid c Hge).
 Qed.
@@ -273,6 +368,8 @@ Proof.
   - destruct (op_current st c) as [j'|] eqn:Hc; try discriminate.
     destruct (Nat.eqb j' j0) eqn:Ej; try discriminate.
     inversion Hcur; subst. eapply Hadm; eauto.
+  - eapply Hadm; eauto.
+  - eapply Hadm; eauto.
   - eapply Hadm; eauto.
   - destruct Hpre as [Hdispatch_lt Hdispatch_adm].
     destruct (Nat.eqb c c0) eqn:Ecc.
@@ -296,9 +393,6 @@ Proof.
   destruct Hinv as [Hstruct Hidle Hadm].
   constructor.
   - eapply op_step_preserves_struct_inv; eauto.
-    intros c j Heq.
-    subst ev.
-    exact Hrange.
   - eapply op_step_preserves_idle_outside_range; eauto.
   - eapply op_step_preserves_admissibility; eauto.
 Qed.
